made progress on sanity proof

Chick.v
@@ -1,8 +1,11 @@
 Set Implicit Arguments.
 
 From Coq Require Import
+     Ascii
      List
+     NPeano
      Program
+     Recdef
      String
      Unicode.Utf8
 .
@@ -40,7 +43,7 @@ Global Instance Desc_TypeD : Desc TypeD:=
   }.
 
 Notation "a --> b" := (ArrowD a b) (at level 99, right associativity).
-Notation "[ a ]" := (ListD a).
+Notation "[ a ]d" := (ListD a).
 
 Check List.fold_left.
 
@@ -48,10 +51,10 @@ Inductive OpD : TypeD -> Type :=
 | EvenD : OpD ( NatD --> BoolD )
 | FoldLeftD :
     ∀ (A B : TypeD) (f : OpD (A --> B --> A)) (base : denoteTypeD A),
-      OpD ( [ B ] --> A )
+      OpD ( [ B ]d --> A )
 | MapD :
     ∀ (t1 t2 : TypeD) (f : OpD (t1 --> t2)),
-      OpD ( [ t1 ] --> [ t2 ] )
+      OpD ( [ t1 ]d --> [ t2 ]d )
 .
 
 Fixpoint denote_OpD (d : TypeD) (opD : OpD d) : denoteTypeD d :=
@@ -78,23 +81,23 @@ Qed.
 
 Module δAtom.
 
-  Inductive D (τ : Type) : Type :=
-  | Same    :      D τ
-  | Replace : τ -> D τ
+  Inductive Δ (τ : Type) : Type :=
+  | Same    :      Δ τ
+  | Replace : τ -> Δ τ
   .
   Arguments Same [τ].
 
-  Definition patch τ (d : D τ) : τ -> option τ :=
-    match d with
+  Definition patch τ (δ : Δ τ) : τ -> option τ :=
+    match δ with
     | Same      => Some
     | Replace r => fun _ => Some r
     end.
 
-  Global Instance Desc_D τ : Desc (D τ) :=
+  Global Instance Desc_Δ τ : Desc (Δ τ) :=
     {
       To := τ -> τ;
-      denote d :=
-        match d with
+      denote δ :=
+        match δ with
         | Same      => id
         | Replace r => fun _ => r
         end;
@@ -104,123 +107,71 @@ End δAtom.
 
 Module δList.
 
-  Inductive D (τ : Type) : Type :=
-  | Same   : D τ
-  | Insert : ∀ (h  : τ)         (δt : D τ), D τ
-  | Modify : ∀ (δh : δAtom.D τ) (δt : D τ), D τ
+  Inductive Δ (τ : Type) (Δτ : Type) : Type :=
+  | Same   : Δ τ Δτ
+  | Insert : ∀ (h  : τ)  (Δt : Δ τ Δτ), Δ τ Δτ
+  | Modify : ∀ (Δh : Δτ) (Δt : Δ τ Δτ), Δ τ Δτ
   .
-  Arguments Same [τ].
+  Arguments Same [τ Δτ].
 
-  Fixpoint patch τ (d : D τ) : list τ -> option (list τ) :=
-    match d with
+  Fixpoint patch τ Δτ (patchτ : Δτ -> τ -> option τ)
+           (δ : Δ τ Δτ) : list τ -> option (list τ) :=
+    match δ with
     | Same         => Some
-    | Insert h  δt => fun l => option_map (cons h) (patch δt l)
+    | Insert h  δt => fun l => option_map (cons h) (patch patchτ δt l)
     | Modify δh δt =>
       fun l =>
         match l with
         | []     => None
-        | h :: t => option_map (cons (⟦ δh ⟧ h)) (patch δt t)
+        | h :: t =>
+          match (patchτ δh h, patch patchτ δt t) with
+          | (Some h', Some t') => Some (h' :: t')
+          | _ => None
+          end
         end
     end.
 
-  Global Instance Desc_D τ : Desc (D τ) :=
-    {
-      To := list τ -> option (list τ);
-      denote := @patch τ;
-    }.
-
 End δList.
 
-Module δTerm.
-
-  Inductive δ : Type :=
-  | Same : δ
-  .
-
-End δTerm.
-
-Definition insert42 := ⟦ δList.Insert 42 δList.Same ⟧.
-
-Theorem insert42works : insert42 [1; 2; 3] = Some [42; 1; 2; 3].
-Proof.
-  reflexivity.
-Qed.
-
-Theorem mapNatBoolworks :
-  ⟦ MapD EvenD ⟧ [0; 1; 2; 3] = [true; false; true; false].
-Proof.
-  reflexivity.
-Qed.
-
-Theorem thm1 :
-  ∀ T (x : T) l,
-    ⟦ δList.Insert x δList.Same⟧ l = Some (x :: l).
-Proof.
-  reflexivity.
-Qed.
-
-Theorem thm2 :
-  ∀
-    (A B : TypeD) (f : OpD (A --> B)) x l,
-    Some (⟦ MapD f ⟧ (x :: l)) = Some (⟦ f ⟧ x :: ⟦ MapD f ⟧ l).
-Proof.
-  induction l.
-  + reflexivity.
-  + now reflexivity.
-Qed.
-
-Theorem option_map_compose :
-  ∀ A B C (f1 : A -> B) (f2 : B -> C) x,
-    option_map f2 (option_map f1 x) = option_map (f2 ∘ f1) x.
-Proof.
-  now destruct x.
-Qed.
-
-Theorem thm3 :
-  ∀ (A B : TypeD) (f : OpD (A --> B)) (x : denoteTypeD A) δl l,
-    option_map
-      ⟦ MapD f ⟧
-      (⟦ δList.Insert x δl ⟧ l)
-    =
-    option_map
-      (cons (⟦ f ⟧ x) ∘ ⟦ MapD f ⟧)
-      (⟦ δl ⟧ l).
-Proof.
-  induction l; simpl; now rewrite option_map_compose. (* damn Coq! *)
-Qed.
-
-Record δ (d : TypeD) :=
+Record Δ (D : TypeD) :=
   {
     δτ : Type;
-    patch : δτ -> denoteTypeD d -> option ⟦ d ⟧
+    patch : δτ -> denoteTypeD D -> option ⟦ D ⟧
   }.
 
-(*
-Definition δArrowD d1 d2 : δ (ArrowD d1 d2).
-  refine {| δτ := False; patch := _; |}.
-  destruct 1.
-Defined.
-*)
-
-Definition δBoolD : δ BoolD.
-  apply Build_δ with (δτ := δAtom.D bool).
+Definition δBoolD : Δ BoolD.
+  apply Build_Δ with (δτ := δAtom.Δ bool).
   apply δAtom.patch.
 Defined.
 
 Definition Variable' := string.
-Definition Binder := option Variable'.
+Definition Binder ν := option ν.
 
 Inductive Term (ν : Type) : Type :=
 | App   : ∀ (t1 t2 : Term ν), Term ν
-| Pi    : ∀ (τ1 : Term ν) (b : Binder) (τ2 : Term ν), Term ν
+| Pi    : ∀ (τ1 : Term ν) (b : Binder ν) (τ2 : Term ν), Term ν
 | Type' : Term ν
 | Var   : ∀ (v : ν), Term ν
 .
 Arguments Type' [ν].
 
+Definition mkApp a t : Term Variable' := App a t.
+
 Definition mkPi '(b, τ) a : Term Variable' := Pi τ b a.
 
+Definition foldlWith T A f (l : list T) (a : A) := List.fold_left f l a.
+
 Definition foldrWith T A f (l : list T) (a : A) := List.fold_right f a l.
+
+Definition applyTerm := foldlWith mkApp.
+
+Definition VTerm ν := (ν * Term ν)%type.
+Definition VTerms ν := list (VTerm ν).
+Definition BTerm ν := (Binder ν * Term ν)%type.
+Definition BTerms ν := list (BTerm ν).
+
+Definition applyVar (l : VTerms Variable') : Term Variable' -> Term Variable' :=
+  applyTerm (List.map (@Var _ ∘ fst) l).
 
 Definition quantifyBinders := foldrWith mkPi.
 
@@ -229,9 +180,7 @@ Definition quantifyVariables l : Term Variable' -> Term Variable' :=
 
 Notation "f $ x" := (f x) (right associativity, at level 180, only parsing).
 
-Definition VTerms := list (Variable' * Term Variable').
-
-Definition mkMotiveType' indName (indParams indIndices : VTerms) universe :=
+Definition mkMotiveType' indName (indParams indIndices : VTerms Variable') universe :=
 
   let onIndIndexOutside '(v, p) t       := Pi  p (Some v) t      in
   let onIndParam        t       '(b, _) := App t (Var b) in
@@ -254,33 +203,472 @@ Definition mkMotiveType' indName (indParams indIndices : VTerms) universe :=
     indIndices
 .
 
-Definition mkCase motive consName consParameters consIndices :=
-  quantifyBinders (concatMap addRecursiveMotive consParameters)
-                  $ applyTerm [applyVar consParameters (Var Nothing consName)]
+Fixpoint unpackFullyAppliedInductive' inductiveName term nbParams nbIndices acc :=
+  match (term, nbParams, nbIndices) with
+  | (Var v, 0, 0) =>
+    if string_dec v inductiveName
+    then Some acc
+    else None
+  | (_, 0, 0) => None
+  | (App l _, _, 0) =>
+    unpackFullyAppliedInductive' inductiveName l (nbParams - 1) nbIndices       acc
+  | (App l r, _, _) =>
+    unpackFullyAppliedInductive' inductiveName l nbParams       (nbIndices - 1) (r :: acc)
+  | (_, _, _) => None
+  end.
+
+Definition unpackFullyAppliedInductive
+           (inductiveName : string)
+           (inductiveParameters : VTerms Variable')
+           (inductiveIndices : VTerms Variable')
+           t :=
+  unpackFullyAppliedInductive' inductiveName t
+                               (List.length inductiveParameters)
+                               (List.length inductiveIndices)
+                               [].
+
+Definition addRecursiveMotive
+           inductiveName inductiveParameters inductiveIndices motive (vτ : VTerm Variable')
+  : BTerms Variable' :=
+  let '(v, τ) := vτ in
+  match unpackFullyAppliedInductive inductiveName inductiveParameters inductiveIndices τ with
+  | Some indices =>
+    [ (Some v, τ)
+    ; (None, App (applyTerm indices motive) (Var v))
+    ]
+  | None => [(Some v, τ)]
+  end.
+
+Definition mkCase
+           inductiveName inductiveParameters inductiveIndices motive consName consParameters
+           consIndices :=
+  quantifyBinders (flat_map
+                     (addRecursiveMotive inductiveName inductiveParameters inductiveIndices motive)
+                     consParameters)
+                  $ applyTerm [applyVar consParameters (Var consName)]
                   $ applyTerm consIndices
                   $ motive.
 
-Definition quantifyCase motive (constructor : (Variable' * VTerms * list (Term Variable'))) acc :=
+Definition quantifyCase
+           inductiveName inductiveParameters inductiveIndices motive
+           (constructor : (Variable' * VTerms Variable' * list (Term Variable'))) acc :=
   let '(consName, consParameters, consIndices) := constructor in
-  Pi (mkCase motive consName consParameters consIndices) None acc.
+  Pi (mkCase inductiveName inductiveParameters inductiveIndices motive
+             consName consParameters consIndices) None acc.
 
-Definition quantifyCases motive (constructors : list (Variable' * VTerms * list (Term Variable'))) :=
-  foldrWith (quantifyCase motive) constructors.
+Definition quantifyCases
+           inductiveName inductiveParameters inductiveIndices motive
+           (constructors : list (Variable' * VTerms Variable' * list (Term Variable'))) :=
+  foldrWith (quantifyCase inductiveName inductiveParameters inductiveIndices motive) constructors.
 
 Definition eliminatorType'
            (inductiveName       : Variable')
-           (inductiveParameters : VTerms)
-           (inductiveIndices    : VTerms)
-           (constructors        : list (Variable' * VTerms * list (Term Variable')))
+           (inductiveParameters : VTerms Variable')
+           (inductiveIndices    : VTerms Variable')
+           (constructors        : list (Variable' * VTerms Variable' * list (Term Variable')))
   :=
 
-  let motive := "Motive" in
-  let motiveType := mkMotiveType' inductiveName inductiveParameters inductiveIndices Type' in
+    let discriminee := "instance" in
+    let discrimineeTerm := Var discriminee in
+    let discrimineeType := applyVar inductiveIndices
+                                    $ applyVar inductiveParameters
+                                    $ Var inductiveName
+    in
+
+    let motive := "Motive" in
+    let motiveTerm := Var motive in
+    let motiveType := mkMotiveType' inductiveName inductiveParameters inductiveIndices Type' in
+
+    let outputType := App (applyVar inductiveIndices motiveTerm) discrimineeTerm in
 
     quantifyVariables inductiveParameters
-  $ quantifyVariables ([(motive, motiveType)])
-  $ quantifyCases motive constructors
-  $ quantifyVariables inductiveIndices
-  $ quantifyVariables [(discriminee, discrimineeType)]
-  $ outputType
+                      $ quantifyVariables ([(motive, motiveType)])
+                      $ quantifyCases inductiveName inductiveParameters inductiveIndices motiveTerm
+                      constructors
+                      $ quantifyVariables inductiveIndices
+                      $ quantifyVariables [(discriminee, discrimineeType)]
+                      $ outputType
 .
+
+Inductive Constructor ν :=
+  { constructorName       : ν
+  ; constructorParameters : BTerms ν
+  ; constructorIndices    : list (Term ν)
+  }.
+
+Inductive Inductive' ν :=
+  { inductiveName         : ν
+  ; inductiveParameters   : VTerms ν
+  ; inductiveIndices      : BTerms ν
+  ; inductiveConstructors : list (Constructor ν)
+  }.
+
+Definition mapWithIndex (A B : Type) (f : A -> nat -> B) (l : list A) : list B :=
+  fst $ List.fold_right (fun a '(acc, i) => (f a i :: acc, i + 1)) ([], 0) l.
+
+Definition digit_of_nat n := ascii_of_nat (n + 48).
+
+Function string_of_nat_aux n acc {measure (fun x => x) n} :=
+  match n with
+    | 0 => acc
+    | _ => string_of_nat_aux (n / 10) (String (digit_of_nat (n mod 10)) acc)
+  end.
+Proof.
+  intros. apply Nat.div_lt; auto with arith.
+Defined.
+
+Definition string_of_nat n :=
+  match n with
+    | 0 => "0"%string
+    | _ => string_of_nat_aux n EmptyString
+  end.
+
+Definition instantiateBinders prefix : BTerms Variable' -> VTerms Variable' :=
+  let instantiate x i :=
+      match x with
+      | (Some v , τ) => (v, τ)
+      | (None,    τ) => (String.append prefix (string_of_nat i), τ)
+      end
+  in
+  mapWithIndex instantiate.
+
+
+Definition instantiateConstructor '(Build_Constructor cn cps cis) :=
+  (cn, instantiateBinders "p" cps, cis).
+
+Definition instantiateConstructors := List.map instantiateConstructor.
+
+Definition eliminatorType (ind : Inductive' Variable') : Term Variable' :=
+  let '(Build_Inductive' indName indParams indIndices indConstructors) := ind in
+
+  eliminatorType' indName indParams
+                  (instantiateBinders "i" indIndices)
+                  (instantiateConstructors indConstructors).
+
+Module δPair.
+
+  Inductive Δ (Δl Δr : Type) : Type :=
+  | Same   : Δ Δl Δr
+  | Modify : ∀ (δl : Δl) (δr : Δr), Δ Δl Δr
+  .
+  Arguments Same [Δl Δr].
+
+  Definition patch Δl Δr
+    (L : Type) (patchL : Δl -> L -> option L)
+    (R : Type) (patchR : Δr -> R -> option R)
+    (δ : Δ Δl Δr) : (L * R) -> option (L * R) :=
+    match δ with
+    | Same         => Some
+    | Modify δl δr =>
+      fun '(l, r) =>
+        match (patchL δl l, patchR δr r) with
+        | (Some l', Some r') => Some (l', r')
+        | _ => None
+        end
+    end.
+
+End δPair.
+
+Module δTerm.
+
+  Inductive Δ (ν : Type) : Type :=
+  | CpyPi   : ∀ (δl : Δ ν) (δb : δAtom.Δ (Binder ν)) (δr : Δ ν), Δ ν
+  | InsPi   : ∀ (δl : Δ ν) (b : Binder ν) (δr : Δ ν), Δ ν
+  | Replace : ∀ (r : Term ν), Δ ν
+  | Same    : Δ ν
+  .
+  Arguments Same [ν].
+
+  Fixpoint patch ν (δ : Δ ν) : Term ν -> option (Term ν) :=
+    match δ with
+
+    | CpyPi δl δb δr =>
+      fun t =>
+        match t with
+        | Pi l b r =>
+          match (patch δl l, δAtom.patch δb b, patch δr r) with
+          | (Some l', Some b', Some r') => Some (Pi l' b' r')
+          | _ => None
+          end
+        | _ => None
+        end
+
+    | InsPi δl b δr =>
+      fun t =>
+        match (patch δl t, patch δr t) with
+        | (Some l', Some r') => Some (Pi l' b r')
+        | _ => None
+        end
+
+    | Replace r => fun _ => Some r
+
+    | Same => Some
+
+    end.
+
+End δTerm.
+
+Module δConstructor.
+
+  Definition Δcn := δAtom.Δ Variable'.
+
+  Definition τcp := BTerm Variable'.
+  Definition Δcp := δPair.Δ (δAtom.Δ (Binder Variable')) (δTerm.Δ Variable').
+  Definition Δcps := δList.Δ τcp Δcp.
+
+  Definition τci := Term Variable'.
+  Definition Δci := δTerm.Δ Variable'.
+  Definition Δcis := δList.Δ τci Δci.
+
+  Inductive Δ :=
+  | Same : Δ
+  | Modify : ∀ (δcn : Δcn) (δcps : Δcps) (δcis : Δcis), Δ
+  .
+
+  Definition patchName (δcn : Δcn) cn := δAtom.patch δcn cn.
+
+  Definition patchParameter : Δcp -> τcp -> option τcp :=
+    δPair.patch (@δAtom.patch _) (@δTerm.patch _).
+
+  Definition patchParameters (δcps : Δcps) cps :=
+    δList.patch patchParameter δcps cps.
+
+  Definition patchIndex : Δci -> τci -> option τci := @δTerm.patch _.
+
+  Definition patchIndices (δcis : Δcis) cis :=
+    δList.patch patchIndex δcis cis.
+
+  Definition patch (δ : Δ) : Constructor Variable' -> option (Constructor Variable') :=
+    match δ with
+    | Same => Some
+    | Modify δcn δcps δcis =>
+      fun '(Build_Constructor cn cps cis) =>
+        match (patchName δcn cn, patchParameters δcps cps, patchIndices δcis cis) with
+        | (Some cn', Some cps', Some cis') => Some (Build_Constructor cn' cps' cis')
+        | _ => None
+        end
+    end.
+
+End δConstructor.
+
+Definition concatListOption A (l : list (option A)) : option (list A) :=
+  List.fold_right
+    (fun oe ol =>
+       match (ol, oe) with
+       | (Some l, Some e) => Some (e :: l)
+       | _ => None
+       end
+    ) (Some []) l.
+
+Module δInductive.
+
+  Definition Δn := δAtom.Δ Variable'.
+
+  Definition τp := VTerm Variable'.
+  Definition Δp := δPair.Δ (δAtom.Δ Variable') (δTerm.Δ Variable').
+  Definition Δps := δList.Δ τp Δp.
+
+  Definition τi := BTerm Variable'.
+  Definition Δi := δPair.Δ (δAtom.Δ (Binder Variable')) (δTerm.Δ Variable').
+  Definition Δis := δList.Δ τi Δi.
+
+  Definition τc := Constructor Variable'.
+  Definition Δc := δConstructor.Δ.
+  Definition Δcs := δList.Δ τc Δc.
+
+  Inductive Δ :=
+  | Same : Δ
+  | Modify : ∀ (δn : Δn) (δps : Δps) (δis : Δis) (δcs : Δcs), Δ
+  .
+
+  Definition patchName (δn : Δn) n := δAtom.patch δn n.
+
+  Definition patchParameter : Δp -> τp -> option τp :=
+    δPair.patch (@δAtom.patch _) (@δTerm.patch _).
+  Definition patchParameters (δps : Δps) ps :=
+    δList.patch patchParameter δps ps.
+
+  Definition patchIndex : Δi -> τi -> option τi :=
+    δPair.patch (@δAtom.patch _) (@δTerm.patch _).
+  Definition patchIndices (δis : Δis) is :=
+    δList.patch patchIndex δis is.
+
+  Definition patchConstructor : Δc -> τc -> option τc :=
+    δConstructor.patch.
+  Definition patchConstructors (δcs : Δcs) cs :=
+    δList.patch patchConstructor δcs cs.
+
+  Definition patch (δ : Δ) : Inductive' Variable' -> option (Inductive' Variable') :=
+    match δ with
+    | Same => Some
+    | Modify δn δps δis δcs =>
+      fun '(Build_Inductive' n ps is cs) =>
+        match
+          (patchName δn n, patchParameters δps ps,
+           patchIndices δis is, patchConstructors δcs cs)
+        with
+        | (Some n', Some ps', Some is', Some cs') =>
+          Some (Build_Inductive' n' ps' is' cs')
+        | _ => None
+        end
+    end.
+
+End δInductive.
+
+Axiom TODO : string -> δTerm.Δ Variable'.
+
+Fixpoint nCpyPis ν n (b : δTerm.Δ ν) : δTerm.Δ ν :=
+  match n with
+  | 0 => b
+  | S n' => δTerm.CpyPi δTerm.Same δAtom.Same (nCpyPis n' b)
+  end.
+
+Fixpoint δquantifyParameters
+         (δps : δInductive.Δps) (ps : VTerms Variable') (rest : δTerm.Δ Variable')
+  : δTerm.Δ Variable'
+  :=
+  match δps with
+  | δList.Insert (b, τ) δps =>
+    δTerm.InsPi (δTerm.Replace τ) (Some b) (δquantifyParameters δps ps rest)
+  | δList.Modify _ _ => TODO "δList.Modify"
+  | δList.Same => nCpyPis (List.length ps) rest
+  end.
+
+Definition δeliminatorType
+           (ind : Inductive' Variable') (δ : δInductive.Δ) : δTerm.Δ Variable' :=
+  let '(Build_Inductive' n ps is cs) := ind in
+  match δ with
+  | δInductive.Same => δTerm.Same
+  | δInductive.Modify δn δps δis δcs =>
+    (* The outermost thing that happens is quantifying over the inductive parameters *)
+    δquantifyParameters δps ps
+                        $ δTerm.CpyPi δTerm.Same δAtom.Same
+                        $ TODO "δInductive.Modify"
+  end.
+
+Theorem option_map_id : forall T (o : option T), option_map id o = o.
+Proof.
+  intros. destruct o; reflexivity.
+Qed.
+
+Theorem nCpyPis_quantifyVariables :
+  ∀ l δrest rest,
+    δTerm.patch (nCpyPis (List.length l) δrest) (quantifyVariables l rest)
+    = option_map (quantifyVariables l) (δTerm.patch δrest rest).
+Proof.
+  induction l; intros.
+  - simpl.
+    unfold quantifyVariables.
+    simpl.
+    unfold quantifyBinders.
+    unfold foldrWith.
+    simpl.
+    rewrite option_map_id.
+    reflexivity.
+  - destruct a as (v, t).
+    simpl.
+    unfold quantifyVariables in IHl.
+    rewrite IHl.
+    destruct (δTerm.patch δrest rest)eqn:PREST; simpl.
+    + unfold quantifyVariables.
+      simpl.
+      reflexivity.
+    + reflexivity.
+Qed.
+
+Theorem option_map_Some : forall A B (f : A -> B) x y,
+  option_map f x = Some y ->
+  exists inside, x = Some inside /\ f inside = y.
+Proof.
+  intros.
+  destruct x as [some|].
+  - exists some. simpl in *. split; congruence.
+  - simpl in H. congruence.
+Qed.
+
+Theorem δquantifyParameters_correct :
+  ∀ δps ps ps',
+    δInductive.patchParameters δps ps = Some ps' ->
+    ∀ δrest rest rest',
+      δTerm.patch δrest rest = Some rest' ->
+      δTerm.patch (δquantifyParameters δps ps δrest) (quantifyVariables ps rest)
+      = Some (quantifyVariables ps' rest').
+Proof.
+  unfold δInductive.patchParameters.
+  intros δps.
+  induction δps; intros ps ps' HI δrest rest rest' HT; simpl in *.
+
+  - rewrite nCpyPis_quantifyVariables.
+    rewrite HT.
+    simpl.
+    congruence.
+
+  - destruct h as (b, τ).
+    apply option_map_Some in HI.
+    destruct HI as [ps'' [HI1 HI2]].
+    subst ps'.
+    simpl in *.
+    erewrite IHδps; try eassumption.
+    unfold quantifyVariables.
+    simpl.
+    reflexivity.
+
+  - admit.
+
+Admitted.
+
+Theorem δeliminatorType_correct : ∀ i δi δt,
+    δeliminatorType i δi = δt ->
+    ∀ t i' t',
+      eliminatorType i = t ->
+      δInductive.patch δi i = Some i' ->
+      δTerm.patch δt t = Some t' ->
+      eliminatorType i' = t'.
+Proof.
+  intros i δi δt Hδe t i' t' He HδI HδT.
+  destruct i as [n ps is cs].
+  destruct i' as [n' ps' is' cs'].
+  simpl in *.
+  destruct δi; simpl in *.
+
+  - inversion HδI; subst; clear HδI.
+    simpl in HδT.
+    inversion HδT; subst.
+    reflexivity.
+
+  - destruct (δInductive.patchName         δn   n)eqn:PN;  [ | congruence ].
+    destruct (δInductive.patchParameters   δps ps)eqn:PPS; [ | congruence ].
+    destruct (δInductive.patchIndices      δis is)eqn:PIS; [ | congruence ].
+    destruct (δInductive.patchConstructors δcs cs)eqn:PCS; [ | congruence ].
+    inversion HδI; subst; clear HδI.
+    unfold eliminatorType' in *.
+
+    erewrite δquantifyParameters_correct in HδT; try eassumption;
+      [ inversion_clear HδT; reflexivity | ].
+
+    TODO: WORKING ON THIS BELOW
+
+Theorem δquantifyMotive_correct :
+  ∀ δps ps ps',
+    δInductive.patchParameters δps ps = Some ps' ->
+    ∀ δrest rest rest',
+      δTerm.patch δrest rest = Some rest' ->
+      δTerm.patch (δquantifyParameters δps ps δrest) (quantifyVariables ps rest)
+      = Some (quantifyVariables ps' rest').
+Proof.
+  unfold δInductive.patchParameters.
+  intros δps.
+  induction δps; intros ps ps' HI δrest rest rest' HT; simpl in *.
+
+
+
+
+    simpl.
+
+    *
+      eapply H0. eassumption.
+    * admit.
+
+    * admit.
+
+Admitted.
